WIP: poly_tobytes correctness proof; general cleanup and proof updates

proof/correctness/avx2/KyberPoly_avx2_proof.ec
@@ -6,6 +6,7 @@ require import AVX2_Ops.
 require import Kyber_AVX2_cf.
 require import KyberCPA_avx2.
 require import KyberPoly_avx2_prevec.
+require import NTT_avx2.
 require import Fq_avx2.
 require import Fq.
 require import NTT_Fq.
@@ -120,40 +121,8 @@ import SignedReductions.
 import Zq.
 import ZModP.
 import Fq_avx2.
-
-op signed_bound_cxq(coefs : W16.t Array256.t, l u c : int) : bool =
-  forall k, l <= k < u => b16 coefs.[k] (c*q).
-
-op pos_bound256_cxq (coefs : W16.t Array256.t) (l u c : int) : bool =
-  forall (k : int), l <= k < u => bpos16 coefs.[k] (c * q).
-
-op pos_bound256_b (coefs : W16.t Array256.t) (l u b : int) : bool =
-  forall (k : int), l <= k < u => bpos16 coefs.[k] b.
-
-op lift_array256 (p: W16.t Array256.t) =
-  Array256.map (fun x => inFq (W16.to_sint x)) p.
-
-op lift_array128 (p: W16.t Array128.t) =
-  Array128.map (fun x => inFq (W16.to_sint x)) p.
-
-lemma lift_array256E (x : W16.t Array256.t) k :
-  0 <= k < 256 =>
-  (lift_array256 x).[k] = inFq (to_sint x.[k]).
-proof. admit. (*  by move => ?; rewrite /lift_array256 mapiE //. *)qed.
-
-lemma lift_array256P (x y : W16.t Array256.t) :
-  lift_array256 x = lift_array256 y <=>
-  (forall k, 0 <= k < 256 => inFq (to_sint x.[k]) = inFq (to_sint y.[k])).
-proof. admit. (*
-  split; first by rewrite tP => H *; rewrite -!lift_array256E // H //.
-  by rewrite tP => H *; rewrite !lift_array256E // H //.
-*)qed.
-
-op touches (m m' : global_mem_t) (p : address) (len : int) =
-    forall i, !(0 <= i < len) => m'.[p + i] = m.[p + i]. (* FIXME: merge w/ KyberPoly *)
-
-op load_array32(m : global_mem_t, p : address) : W8.t Array32.t = 
-      Array32.init (fun i => m.[p + i]).
+import NTT_Avx2.
+import KyberPoly.
 
 lemma get_lift_array256_eq (p: W16.t Array256.t):
   let p_lift = lift_array256 p in
@@ -163,6 +132,11 @@ proof. admit. (*
   move => k k_i.
   smt (@Array256).
 *)qed.
+
+lemma lift_array256E (x : W16.t Array256.t) k :
+  0 <= k < 256 =>
+  (lift_array256 x).[k] = inFq (to_sint x.[k]).
+proof. admit. (*  by move => ?; rewrite /lift_array256 mapiE //. *)qed.
 
 lemma poly_add_corr_h _a _b ab bb :
       0 <= ab <= 6 => 0 <= bb <= 3 =>
@@ -363,57 +337,6 @@ lemma poly_sub_corr _a _b ab bb :
               inFq (to_sint res.[k]) = _a.[k] - _b.[k]] = 1%r
   by move => *; conseq poly_sub_ll (poly_sub_corr_h _a _b ab bb _ _).
 
-
-(* FIXME: dup from KyberPoly*)
-lemma m1true x :
-  0 <= x < 16 =>
-    (W16.of_int 65535).[x].
-proof. admit. (*
-  move => *.
-  rewrite of_intwE => />.
-  rewrite /int_bit => />.
-  case (x = 0); first by smt(@Ring.IntID) => />.
-  move => *; case(x=1); first by auto => />.
-  move => *; case(x=2); first by auto => />.
-  move => *; case(x=3); first by auto => />.
-  move => *; case(x=4); first by auto => />.
-  move => *; case(x=5); first by auto => />.
-  move => *; case(x=6); first by auto => />.
-  move => *; case(x=7); first by auto => />.
-  move => *; case(x=8); first by auto => />.
-  move => *; case(x=9); first by auto => />.
-  move => *; case(x=10); first by auto => />.
-  move => *; case(x=11); first by auto => />.
-  move => *; case(x=12); first by auto => />.
-  move => *; case(x=13); first by auto => />.
-  move => *; case(x=14); first by auto => />.
-  move => *; case(x=15); first by auto => />.
-  smt().
-*)qed.
-
-lemma getsign x :
-      (x \slt W16.zero => x `|>>` (of_int 15)%W8 = (of_int 65535)%W16) /\
-      (W16.zero \sle x => x `|>>` (of_int 15)%W8 = W16.zero).
-proof. admit. (*
-  rewrite /(`|>>`) sarE sltE sleE !to_sintE /smod => />.
-  split; move => hh.
-    have  xb : (32768 <= to_uint x); first by smt(W16.to_uint_cmp).
-    apply W16.ext_eq => k kb; rewrite initiE => />.
-    rewrite (_: min 15 (k+15) = 15); first by smt().
-    by rewrite m1true // get_to_uint => />;smt().
-  have  xb : (0 <= to_uint x < 32768).
-     split; first by smt().
-     case (32768 <= to_uint x).
-        move => *.
-        have ? : false;  move : (W16.to_uint_cmp x) => />; smt().
-        smt().
-  move => *.
-    apply W16.ext_eq => k kb; rewrite initiE => />.
-    rewrite (_: min 15 (k+15) = 15); first by smt().
-    by rewrite get_to_uint => />;smt().
-*)qed.
-
-
 lemma poly_csubq_corr_h ap :
       hoare[ Mprevec.poly_csubq :
              ap = lift_array256 rp /\
@@ -454,9 +377,10 @@ proof. admit. (*
   auto => />.
   move => &hr [#] *.
   case (_r{hr}.[k] \slt W16.zero).
-    + smt(getsign @Array16 @W16).
-    + rewrite W16.sltE ltzNge -W16.sleE => /=.
-      smt(getsign @Array16 @W16).
+    + rewrite initiE 1://= /= -/(W16.onew).
+      apply getsignNeg.
+    + rewrite W16.sltE ltzNge -W16.sleE initiE 1://= /=.
+      apply getsignPos.
   auto => />.
   move => &hr [#] *.
   do split.
@@ -1278,11 +1202,6 @@ proof. admit. (*
   + inline *; wp; auto => /> /#.
 *)qed.
 
-op load_array128(m : global_mem_t, p : address) : W8.t Array128.t = 
-      Array128.init (fun i => m.[p + i]).
-
-op valid_ptr(p : int, o : int) = 0 <= o => 0 <= p /\ p + o < W64.modulus.
-
 lemma poly_decompress_corr mem _p (_a : W8.t Array128.t): 
     equiv [ Mprevec.poly_decompress ~ EncDec_AVX2.decode4 :
              valid_ptr _p 128 /\
@@ -1391,14 +1310,21 @@ proof. admit. (*
           congr.
           rewrite /round_scalew /round => />.
           rewrite /truncateu16.
+          rewrite /wmulls => />.
+          rewrite /truncateu16.
+          rewrite of_uintK.
           rewrite shift_def 1:/# q_def 1:/# mask_def 1:/# modz_dvd //.
           rewrite (W16.of_sintK 3329) /smod //= of_sintK.
+          pose b := pack2_t (W2u8.Pack.init (fun (_ : int) => mem.[to_uint (ap{1} + (of_int (8 * i{2}))%W64) + 2 * (k %% 16) %/ 4])).
           case ((k %% 2) = 0) => k_even.
             + rewrite (_: pc_mask_s = (W16.of_int (2^4 - 1))). simplify. done.
               rewrite W16.and_mod 1://.
               rewrite /q.
-              pose b := pack2_t (W2u8.Pack.init (fun (_ : int) => mem.[to_uint (ap{1} + (of_int (8 * i{2}))%W64) + 2 * (k %% 16) %/ 4])).
-              rewrite of_intM of_sintK.
+              rewrite of_sintK.
+              rewrite (W16.of_sintK 2048) //= /(W16.smod 2048) //=.
+              rewrite modz_dvd 1://=.
+              rewrite of_sintK (pmod_small _ W16.modulus). by move : (modz_cmp (to_uint b) 16) => /#.
+              rewrite (_: W16.smod (to_uint b %% 16) = to_uint b %% 2 ^ 4). move : (modz_cmp (to_uint b) 16); rewrite /W16.smod => /#.
               rewrite (_: W16.smod (to_uint b %% 2 ^ 4 * 2048 %% W16.modulus) = to_uint b %% 2 ^ 4 * 2048).
                 rewrite /smod /=.
                 smt(pmod_small @Int @IntDiv @Ring.IntID).
@@ -1420,8 +1346,12 @@ proof. admit. (*
                 smt(@Int @IntDiv).
               rewrite -zeroext_truncateu8_and.
               rewrite to_uint_zeroextu16.
-              rewrite (_: to_uint (truncateu8 b) = to_uint mem.[to_uint (ap{1} + (of_int (8 * i{2}))%W64) + 2 * (k %% 16) %/ 4]).
-                admit. (* FIXME *)
+              rewrite (_: to_uint (truncateu8 b) = to_uint mem.[to_uint (ap{1} + (of_int (8 * i{2}))%W64) + 2 * (k %% 16) %/ 4]). (* can be simplified *)
+                rewrite to_uint_truncateu8 //=.
+                rewrite -(divz1 (to_uint b)) -(Ring.IntID.expr0 2) (_: 0 = 8 * 0) 1://=.
+                rewrite -(W8.of_uintK (to_uint b %/ 2 ^ (8 * 0))) -W2u8.of_int_bits8_div 1://=.
+                rewrite to_uintK.
+                rewrite -get_unpack8 1://= pack2K initiE 1://= //=.
               rewrite (_: 2 * (k %% 16) %/ 4 = k %% 16 %/ 2). smt(@IntDiv @Int).
               rewrite to_uintD of_uintK.
               rewrite (pmod_small (8 * i{2}) W64.modulus). move : i_tub i_lb => /#.
@@ -1430,15 +1360,31 @@ proof. admit. (*
               rewrite (addzC 8 _).
               do (rewrite get_setE 1:/#).
               smt(@Array256).
-            + pose b := pack2_t ((W2u8.Pack.init (fun (_ : int) => mem.[to_uint (ap{1} + (of_int (8 * i{2}))%W64) +
-                                                              2 * (k %% 16) %/ 4]))).
-              rewrite (_: b `&` (W16.of_int 240) = ((b `>>>` 4) `&` (W16.of_int (2^4 - 1))) `<<<` 4).
-                admit. (* FIXME: smt(@Int @IntDiv @W16 and_mod @Ring.IntID @W2u8). *)
+            + rewrite (_: b `&` (W16.of_int 240) = ((b `>>>` 4) `&` (W16.of_int (2^4 - 1))) `<<<` 4). (* can be simplified *)
+                rewrite (_: 2^4 - 1 = 240 %% W16.modulus %/ 2^4). by trivial.
+                rewrite -W16.shrDP 1://= shrw_and shrl_andmaskN 1://= -andwA.
+                rewrite (_: (of_int 240)%W16 `&` invw ((W16.masklsb 4)) = (W16.of_int 240)).
+                  rewrite /invw /max 1://=.
+                  rewrite /of_int /(pc_mask_s).
+                  rewrite W16.wordP => j j_i.
+                    rewrite andwE.
+                    rewrite /bits2w /= /int2bs /= /mkseq /= mapiE 1:j_i /=.
+                    do rewrite initiE 1:j_i /=.
+                    rewrite -iotaredE //=.
+                    smt(@Int @List @Logic).
+                 done.
               rewrite W16.and_mod 1://=.
               rewrite /q.
               rewrite shlMP 1://=.
+              rewrite -to_sintM_small.
+                rewrite (W16.of_sintK 128) /smod //= of_sintK.
+                rewrite (_: W16.smod (to_uint (b `>>>` 4) %% 2 ^ 4 * 2^4 %% W16.modulus) = to_uint (b `>>>` 4) %% 2 ^ 4 * 2^4).
+                  rewrite /smod /=.
+                  smt(pmod_small @Int @IntDiv @Ring.IntID).
+                smt(pmod_small @Int @IntDiv @Ring.IntID).
               rewrite of_intM.
               rewrite (mulzA _ (2^4) 128) //=.
+              rewrite of_sintK.
               rewrite of_sintK.
               rewrite (_: W16.smod (to_uint (b `>>>` 4) %% 16 * 2048 %% W16.modulus) =
                           to_uint (b `>>>` 4) %% 16 * 2048).
@@ -1447,20 +1393,43 @@ proof. admit. (*
                 smt(@Int @IntDiv @Ring.IntID).
               do rewrite shr_shrw 1://=.
               rewrite shrDP 1://=.
-              rewrite (pmod_small _ W32.modulus). by smt(@Int @IntDiv @Ring.IntID).
               rewrite -of_intD shrDP 1://= of_uintK.
-              do (rewrite (pmod_small _ W32.modulus); first by smt(@Int @IntDiv @Ring.IntID)).
-              rewrite (pmod_small _ W16.modulus); first by smt(@Int @IntDiv @Ring.IntID).
+              do (rewrite (modz_dvd _ W32.modulus W16.modulus) 1://=).
+              rewrite (pmod_small (to_uint (b `>>>` 4) %% 16 * 2048) W16.modulus); first by smt(@Int @IntDiv @Ring.IntID).
+              rewrite (_: W16.smod (to_uint (b `>>>` 4) %% 16 * 2048) =
+                          to_uint (b `>>>` 4) %% 16 * 2048).
+                move : (modz_cmp (to_uint (b `>>>` 4)) 16). simplify.
+                rewrite /smod.
+                smt(@Int @IntDiv @Ring.IntID).
+              rewrite (pmod_small (to_uint (b `>>>` 4) %% 16 * 2048 * 3329) W32.modulus); first by smt(@Int @IntDiv @Ring.IntID).
               rewrite (_: to_uint (b `>>>` 4) %% 16 * 2048 * 3329 %/ 2 ^ 14 =  to_uint (b `>>>` 4) %% 16 * 3329 %/ 2 ^ 3).
                 smt(@Int @IntDiv @Ring.IntID).
+              rewrite (pmod_small _ W32.modulus); first by smt(@Int @IntDiv @Ring.IntID).
               rewrite (_: (to_uint (b `>>>` 4) %% 16 * 3329 %/ 2 ^ 3 + 1) %/ 2 ^ 1 = (8 + to_uint (b `>>>` 4) %% 16 * 3329) %/ 2 ^ 4).
                 smt(@Int @IntDiv @Ring.IntID).
+              rewrite (pmod_small _ W16.modulus); first by smt(@Int @IntDiv @Ring.IntID).
               rewrite (_: W16.smod ((8 + to_uint (b `>>>` 4) %% 16 * 3329) %/ 2 ^ 4) = (8 + to_uint (b `>>>` 4) %% 16 * 3329) %/ 2 ^ 4).
                 move : (modz_cmp (to_uint (b `>>>` 4)) 16) => />.
                 rewrite /smod.
                 smt(@Int @IntDiv @Ring.IntID).
-              rewrite (_: (to_uint (b `>>>` 4) %% 16) = to_uint mem.[to_uint (ap{1} + (of_int (8 * i{2}))%W64) + 2 * (k %% 16) %/ 4] %/ 16).
-                admit. (* FIXME *)
+              rewrite (_: (to_uint (b `>>>` 4) %% 16) = to_uint mem.[to_uint (ap{1} + (of_int (8 * i{2}))%W64) + 2 * (k %% 16) %/ 4] %/ 16). (* can be simplified *)
+                rewrite -(pmod_small (to_uint (b `>>>` 4) %% 16) W16.modulus) 1:/#.
+                rewrite -(W16.of_uintK (to_uint (b `>>>` 4) %% 16)).
+                rewrite (_: 16 = 2 ^ 4). by trivial.
+                rewrite -W16.and_mod 1://=.
+                have ->: (W16.of_int (2 ^ 4 - 1)) = W16.masklsb (8 - 4); first by trivial.
+                rewrite -W16.andmask_shrw 1://=.
+                rewrite -(W16.to_uintK' (b `&` (W16.masklsb 8))).
+                rewrite shrDP 1://=.
+                rewrite W16.and_mod 1://= /max //=.
+                rewrite of_uintK of_uintK.
+                rewrite (pmod_small _ W16.modulus); first by smt(@Int @IntDiv @Ring.IntID).
+                rewrite modz_mod.
+                rewrite (pmod_small _ W16.modulus); first by  smt(@Int @IntDiv @Ring.IntID).
+                rewrite -(divz1 (to_uint b)) -(Ring.IntID.expr0 2) (_: 0 = 8 * 0) 1://=.
+                rewrite -(W8.of_uintK (to_uint b %/ 2 ^ (8 * 0))) -W2u8.of_int_bits8_div 1://=.
+                rewrite to_uintK.
+                rewrite -get_unpack8 1://= pack2K initiE 1://= //=.
               rewrite (_: 2 * (k %% 16) %/ 4 = k %% 16 %/ 2). smt(@IntDiv @Int).
               rewrite to_uintD of_uintK.
               rewrite (pmod_small (8 * i{2}) W64.modulus). move : i_tub i_lb => /#.
@@ -1471,22 +1440,30 @@ proof. admit. (*
               smt(@Array256).
         rewrite /round_scalew /round => />.
         rewrite /truncateu16.
-        pose b := pack2_t ((W2u8.Pack.init (fun (_ : int) => mem.[to_uint (ap{1} + (of_int (8 * i{2}))%W64) + 2 * (k %% 16) %/ 4]))).
+        rewrite /wmulls => />.
+        rewrite /truncateu16.
+        rewrite of_uintK.
         rewrite shift_def 1:/# q_def 1:/# mask_def 1:/# modz_dvd //.
-        rewrite (W16.of_sintK 3329) /smod //= of_sintK.
+        rewrite (W16.of_sintK 3329) /(W16.smod 3329) //= of_sintK.
+        pose b := pack2_t ((W2u8.Pack.init (fun (_ : int) => mem.[to_uint (ap{1} + (of_int (8 * i{2}))%W64) + 2 * (k %% 16) %/ 4]))).
         case ((k %% 2) = 0) => k_even.
             + rewrite (_: pc_mask_s = (W16.of_int (2^4 - 1))). simplify. done.
               rewrite W16.and_mod 1://.
               rewrite /q.
-              rewrite of_intM of_sintK.
+              rewrite of_sintK.
+              rewrite (W16.of_sintK 2048) //= /(W16.smod 2048) //=.
+              rewrite modz_dvd 1://=.
+              rewrite of_sintK (pmod_small _ W16.modulus). by move : (modz_cmp (to_uint b) 16) => /#.
+              rewrite (_: W16.smod (to_uint b %% 16) = to_uint b %% 2 ^ 4). move : (modz_cmp (to_uint b) 16); rewrite /W16.smod => /#.
               rewrite (_: W16.smod (to_uint b %% 2 ^ 4 * 2048 %% W16.modulus) = to_uint b %% 2 ^ 4 * 2048).
                 rewrite /smod /=.
                 smt(pmod_small @Int @IntDiv @Ring.IntID).
               do rewrite shr_shrw 1://=.
               rewrite shrDP 1://=.
+              rewrite /(W16.smod 3329) //=.
               rewrite (pmod_small _ W32.modulus). by smt(@Int @IntDiv @Ring.IntID).
               rewrite (_: ((to_uint b %% 2 ^ 4) * 2048 * 3329 %/ 2 ^ 14) = (to_uint b %% 2 ^ 4) * 3329 %/ 2 ^ 3). smt(@Int @IntDiv @Ring.IntID).
-              rewrite -of_intD shrDP 1://= of_uintK.
+              rewrite shrDP 1://= of_uintK.
               do (rewrite (pmod_small _ W32.modulus); first by smt(@Int @IntDiv @Ring.IntID)).
               rewrite (pmod_small _ W16.modulus); first by smt(@Int @IntDiv @Ring.IntID).
               rewrite (_: (to_uint b %% 2 ^ 4 * 3329 %/ 2 ^ 3 + 1) %/ 2 ^ 1 = (8 + to_uint b %% 2 ^ 4 * 3329) %/ 2 ^ 4).
@@ -1498,12 +1475,30 @@ proof. admit. (*
               move : (modz_cmp (to_uint b) 16) => />.
               smt(@Int @IntDiv @Ring.IntID).
             + rewrite (_: b `&` (W16.of_int 240) = ((b `>>>` 4) `&` (W16.of_int (2^4 - 1))) `<<<` 4).
-                admit. (* FIXME: smt(@Int @IntDiv @W16 and_mod @Ring.IntID @W2u8). *)
+                rewrite (_: 2^4 - 1 = 240 %% W16.modulus %/ 2^4). by trivial.
+                rewrite -W16.shrDP 1://= shrw_and shrl_andmaskN 1://= -andwA.
+                rewrite (_: (of_int 240)%W16 `&` invw ((W16.masklsb 4)) = (W16.of_int 240)).
+                  rewrite /invw /max 1://=.
+                  rewrite /of_int /(pc_mask_s).
+                  rewrite W16.wordP => j j_i.
+                    rewrite andwE.
+                    rewrite /bits2w /= /int2bs /= /mkseq /= mapiE 1:j_i /=.
+                    do rewrite initiE 1:j_i /=.
+                    rewrite -iotaredE //=.
+                    smt(@Int @List @Logic).
+                 done.
               rewrite W16.and_mod 1://=.
               rewrite /q.
               rewrite shlMP 1://=.
+              rewrite -to_sintM_small.
+                rewrite (W16.of_sintK 128) /smod //= of_sintK.
+                rewrite (_: W16.smod (to_uint (b `>>>` 4) %% 2 ^ 4 * 2^4 %% W16.modulus) = to_uint (b `>>>` 4) %% 2 ^ 4 * 2^4).
+                  rewrite /smod /=.
+                  smt(pmod_small @Int @IntDiv @Ring.IntID).
+                smt(pmod_small @Int @IntDiv @Ring.IntID).
               rewrite of_intM.
               rewrite (mulzA _ (2^4) 128) //=.
+              rewrite of_sintK.
               rewrite of_sintK.
               rewrite (_: W16.smod (to_uint (b `>>>` 4) %% 16 * 2048 %% W16.modulus) =
                           to_uint (b `>>>` 4) %% 16 * 2048).
@@ -1512,14 +1507,21 @@ proof. admit. (*
                 smt(@Int @IntDiv @Ring.IntID).
               do rewrite shr_shrw 1://=.
               rewrite shrDP 1://=.
-              rewrite (pmod_small _ W32.modulus). by smt(@Int @IntDiv @Ring.IntID).
               rewrite -of_intD shrDP 1://= of_uintK.
-              do (rewrite (pmod_small _ W32.modulus); first by smt(@Int @IntDiv @Ring.IntID)).
-              rewrite (pmod_small _ W16.modulus); first by smt(@Int @IntDiv @Ring.IntID).
+              do (rewrite (modz_dvd _ W32.modulus W16.modulus) 1://=).
+              rewrite (pmod_small (to_uint (b `>>>` 4) %% 16 * 2048) W16.modulus); first by smt(@Int @IntDiv @Ring.IntID).
+              rewrite (_: W16.smod (to_uint (b `>>>` 4) %% 16 * 2048) =
+                          to_uint (b `>>>` 4) %% 16 * 2048).
+                move : (modz_cmp (to_uint (b `>>>` 4)) 16). simplify.
+                rewrite /smod.
+                smt(@Int @IntDiv @Ring.IntID).
+              rewrite (pmod_small (to_uint (b `>>>` 4) %% 16 * 2048 * 3329) W32.modulus); first by smt(@Int @IntDiv @Ring.IntID).
               rewrite (_: to_uint (b `>>>` 4) %% 16 * 2048 * 3329 %/ 2 ^ 14 =  to_uint (b `>>>` 4) %% 16 * 3329 %/ 2 ^ 3).
                 smt(@Int @IntDiv @Ring.IntID).
+              rewrite (pmod_small _ W32.modulus); first by smt(@Int @IntDiv @Ring.IntID).
               rewrite (_: (to_uint (b `>>>` 4) %% 16 * 3329 %/ 2 ^ 3 + 1) %/ 2 ^ 1 = (8 + to_uint (b `>>>` 4) %% 16 * 3329) %/ 2 ^ 4).
                 smt(@Int @IntDiv @Ring.IntID).
+              rewrite (pmod_small _ W16.modulus); first by smt(@Int @IntDiv @Ring.IntID).
               rewrite (_: W16.smod ((8 + to_uint (b `>>>` 4) %% 16 * 3329) %/ 2 ^ 4) = (8 + to_uint (b `>>>` 4) %% 16 * 3329) %/ 2 ^ 4).
                 move : (modz_cmp (to_uint (b `>>>` 4)) 16) => />.
                 rewrite /smod.
@@ -1672,7 +1674,7 @@ proof. admit. (*
       move : (pos_bound_a (64 * i{2} + 48 + k)).
       rewrite (_: 0 <= 64 * i{2} + 48 + k && 64 * i{2} + 48 + k < 256) //=. by move : i_lb i_tub k_lb k_ub => /#.
       rewrite andabP => /(mem_iota 0 3329 (to_sint a{1}.[64 * i{2} + 48 + k])).
-      smt(). (* FIXME *)
+      smt(@Int @IntDiv @Ring.IntID @W16 @Array256).
     + move => k k_lb k_ub.
       do (rewrite initiE /=; first by rewrite k_lb k_ub).
       rewrite compress_alt_nice.
@@ -1719,7 +1721,7 @@ proof. admit. (*
       move : (pos_bound_a (64 * i{2} + 48 + k)).
       rewrite (_: 0 <= 64 * i{2} + 48 + k && 64 * i{2} + 48 + k < 256) //=. by move : i_lb i_tub k_lb k_ub => /#.
       rewrite andabP => /(mem_iota 0 3329 (to_sint a{1}.[64 * i{2} + 48 + k])).
-      smt(). (* FIXME *)
+      smt(@Int @IntDiv @Ring.IntID @W16 @Array256).
     + move => k k_lb k_ub.
       do (rewrite initiE /=; first by rewrite k_lb k_ub).
       rewrite compress_alt_nice.
@@ -1766,7 +1768,7 @@ proof. admit. (*
       move : (pos_bound_a (64 * i{2} + 48 + k)).
       rewrite (_: 0 <= 64 * i{2} + 48 + k && 64 * i{2} + 48 + k < 256) //=. by move : i_lb i_tub k_lb k_ub => /#.
       rewrite andabP => /(mem_iota 0 3329 (to_sint a{1}.[64 * i{2} + 48 + k])).
-      smt(). (* FIXME *)
+      smt(@Int @IntDiv @Ring.IntID @W16 @Array256).
     + move => k k_lb k_ub.
       do (rewrite initiE /=; first by rewrite k_lb k_ub).
       rewrite compress_alt_nice.
@@ -1813,7 +1815,7 @@ proof. admit. (*
       move : (pos_bound_a (64 * i{2} + 48 + k)).
       rewrite (_: 0 <= 64 * i{2} + 48 + k && 64 * i{2} + 48 + k < 256) //=. by move : i_lb i_tub k_lb k_ub => /#.
       rewrite andabP => /(mem_iota 0 3329 (to_sint a{1}.[64 * i{2} + 48 + k])).
-      smt(). (* FIXME *)
+      smt(@Int @IntDiv @Ring.IntID @W16 @Array256).
 
     inline *.
     unroll for {2} 2.
@@ -2078,22 +2080,86 @@ proof. admit. (*
       smt(@Int @IntDiv).
     rewrite shlMP 1://= of_sintK /smod //=.
     rewrite shlMP 1://= of_sintK /smod //=.
+    have f0_b: forall k, 0 <= k < 16 => 0 <= to_sint f0{1}.[k] < 16.
+      move => j j_i.
+      rewrite (f0_def j j_i).
+      apply compress_rng; first by trivial.
+    have f1_b: forall k, 0 <= k < 16 => 0 <= to_sint f1{1}.[k] < 16.
+      move => j j_i.
+      rewrite (f1_def j j_i).
+      apply compress_rng; first by trivial.
+    have f2_b: forall k, 0 <= k < 16 => 0 <= to_sint f2{1}.[k] < 16.
+      move => j j_i.
+      rewrite (f2_def j j_i).
+      apply compress_rng; first by trivial.
+    have f3_b: forall k, 0 <= k < 16 => 0 <= to_sint f3{1}.[k] < 16.
+      move => j j_i.
+      rewrite (f3_def j j_i).
+      apply compress_rng; first by trivial.
     rewrite (_: (if x %% 8 %/ 4 = 0 then f0{1}.[2 * (k %% 8)] \bits8 0
                  else f1{1}.[2 * (k %% 8)] \bits8 0) =
                 (W16.of_int (compress 4 (inFq (to_sint a{1}.[64 * i{2} + 16 * (x %% 8 %/ 4) + 2 * (k %% 8)]))) \bits8 0)).
-      admit. (* FIXME *)
+      case (x %% 8 %/ 4 = 0) => Hx.
+        + rewrite Hx //=.
+          move : (f0_def (2 * (k %% 8))).
+          rewrite mapiE 1:/# //=.
+          move => <-; first by smt().
+          rewrite to_sint_unsigned; first by move : (f0_b (2 * (k %% 8))) => /#.
+          rewrite to_uintK' => //=.
+        + have -> /=: x %% 8 %/ 4 = 1. move : Hx => /#.
+          move : (f1_def (2 * (k %% 8))).
+          rewrite mapiE 1:/# //=.
+          move => <-; first by smt().
+          rewrite to_sint_unsigned; first by move : (f1_b (2 * (k %% 8))) => /#.
+          rewrite to_uintK' => //=.
     rewrite (_: (if x %% 8 %/ 4 = 0 then f0{1}.[2 * (k %% 8) + 1] \bits8 0
                  else f1{1}.[2 * (k %% 8) + 1] \bits8 0) =
                 (W16.of_int (compress 4 (inFq (to_sint a{1}.[64 * i{2} + 16 * (x %% 8 %/ 4) + 2 * (k %% 8) + 1]))) \bits8 0)).
-      admit. (* FIXME *)
+      case (x %% 8 %/ 4 = 0) => Hx.
+        + rewrite Hx //=.
+          move : (f0_def (2 * (k %% 8) + 1)).
+          rewrite mapiE 1:/# //= addzA.
+          move => <-; first by smt().
+          rewrite to_sint_unsigned; first by move : (f0_b (2 * (k %% 8) + 1)) => /#.
+          rewrite to_uintK' => //=.
+        + have -> /=: x %% 8 %/ 4 = 1. move : Hx => /#.
+          move : (f1_def (2 * (k %% 8) + 1)).
+          rewrite mapiE 1:/# //= addzA.
+          move => <-; first by smt().
+          rewrite to_sint_unsigned; first by move : (f1_b (2 * (k %% 8) + 1)) => /#.
+          rewrite to_uintK' => //=.
     rewrite (_: (if x %% 8 %/ 4 = 0 then f2{1}.[2 * (k %% 8)] \bits8 0
                  else f3{1}.[2 * (k %% 8)] \bits8 0) =
                 (W16.of_int (compress 4 (inFq (to_sint a{1}.[64 * i{2} + 32 + 16 * (x %% 8 %/ 4) + 2 * (k %% 8)]))) \bits8 0)).
-      admit. (* FIXME *)
+      case (x %% 8 %/ 4 = 0) => Hx.
+        + rewrite Hx //=.
+          move : (f2_def (2 * (k %% 8))).
+          rewrite mapiE 1:/# //=.
+          move => <-; first by smt().
+          rewrite to_sint_unsigned; first by move : (f2_b (2 * (k %% 8))) => /#.
+          rewrite to_uintK' => //=.
+        + have -> /=: x %% 8 %/ 4 = 1. move : Hx => /#.
+          move : (f3_def (2 * (k %% 8))).
+          rewrite mapiE 1:/# //=.
+          move => <-; first by smt().
+          rewrite to_sint_unsigned; first by move : (f3_b (2 * (k %% 8))) => /#.
+          rewrite to_uintK' => //=.
     rewrite (_: (if x %% 8 %/ 4 = 0 then f2{1}.[2 * (k %% 8) + 1] \bits8 0
                  else f3{1}.[2 * (k %% 8) + 1] \bits8 0) =
                 (W16.of_int (compress 4 (inFq (to_sint a{1}.[64 * i{2} + 32 + 16 * (x %% 8 %/ 4) + 2 * (k %% 8) + 1]))) \bits8 0)).
-      admit. (* FIXME *)
+      case (x %% 8 %/ 4 = 0) => Hx.
+        + rewrite Hx //=.
+          move : (f2_def (2 * (k %% 8) + 1)).
+          rewrite mapiE 1:/# //= addzA.
+          move => <-; first by smt().
+          rewrite to_sint_unsigned; first by move : (f2_b (2 * (k %% 8) + 1)) => /#.
+          rewrite to_uintK' => //=.
+        + have -> /=: x %% 8 %/ 4 = 1. move : Hx => /#.
+          move : (f3_def (2 * (k %% 8) + 1)).
+          rewrite mapiE 1:/# //= addzA.
+          move => <-; first by smt().
+          rewrite to_sint_unsigned; first by move : (f3_b (2 * (k %% 8) + 1)) => /#.
+          rewrite to_uintK' => //=.
     do (rewrite of_int_bits8_div 1://= expr0 divz1).
     have pck_bnds: forall (c1 c2: Fq),
                      0 <= (compress 4 c1) + (compress 4 c2) * 16 < 256.
@@ -2451,9 +2517,13 @@ proof. admit. (*
                                       W8.int_bit (compress_poly 1 (lift_array256 a{1})).[32 * i{2} + 8 * (w %% 4) + j] 0)) (4*i{2}) 4 ra{2}).
     apply Array32.ext_eq => x x_i.
     rewrite filliE 1:x_i //=.
-    case (4 * i{2} <= x && x < 4 * i{2} + 4) => x_si.
+    case (4 * i{2} <= x && x < 4 * i{2} + 4)=> x_si.
       do (rewrite get_setE; first by move : x_si i_lb i_ub => /# //=).
-      (* FIXME: smt should solve *)
+      (* TODO: smt should solve this
+        have Hx: x \in (iota_ (4 * i{2}) 4); first by rewrite mem_iota -andabP x_si.
+        move : Hx.
+        smt(@Int @IntDiv @W32 @List @Array256).
+      *)
       case (x = 4 * i{2} + 3) => x_3.
         by have -> /=: (x %% 4) = 3; move : x_3 => /#.
       case (x = 4 * i{2} + 2) => x_2.
@@ -2491,10 +2561,21 @@ proof. admit. (*
         rewrite modz_pow2_div 1://= //=.
       rewrite (_: 32 * i{2} + 16 * (216 %/ 4 ^ (k %% 4) %% 2) +
                     8 * (216 %/ 4 ^ (k %% 4) %/ 2 %% 2) = 32 * i{2} + 8 * (k %% 4)).
-        have ?: i{2} \in (iota_ 0 8); first by rewrite mem_iota i_tub i_lb.
-        rewrite andabP -(mem_iota (4*i{2}) 4 k) in k_si.
-        move : H k_si.
-        admit. (* FIXME *)
+        ring.
+        (* TODO: smt should solve this
+        have Hi: i{2} \in (iota_ 0 8); first by rewrite mem_iota i_tub i_lb.
+        have Hk: (k %% 4) \in (iota_ 0 4); first by rewrite mem_iota -andabP (modz_cmp k 4).
+        smt(@Int @IntDiv @List @Ring.IntID).
+        *)
+        case (k %% 4 = 0) => k_0.
+          rewrite k_0 //=.
+        case (k %% 4 = 1) => k_1.
+          rewrite k_1 //=.
+        case (k %% 4 = 2) => k_2.
+          rewrite k_2 //=.
+        case (k %% 4 = 3) => k_3.
+          rewrite k_3 //=.
+        move : (modz_cmp k 4) => /#.
 
       do rewrite modz_dvd 1://=.
       rewrite compress_avx2_impl_small 1:pos_bound_a 1:/#.
@@ -2514,11 +2595,11 @@ proof. admit. (*
   smt(@Logic).
   move => mem1 i ra i_tlb _ i_lb i_ub.
   have ->: (i = 8).
-    move : i_tlb i_ub => /#.
-  rewrite /load_array32 /loadW8 => /> mem1_eq_rp mem1_eq_ra.
+    move : i_tlb i_ub => /#. 
+ rewrite /load_array32 /loadW8 => /> mem1_eq_rp mem1_eq_ra.
   apply Array32.ext_eq => x x_i.
   rewrite initiE 1:x_i //= mem1_eq_ra 1:x_i //=.
-*)qed.
+*) qed.
 
 lemma poly_tomsg_ll : islossless  Mprevec.poly_tomsg.
 proc.
@@ -2538,7 +2619,7 @@ lemma bit_decode (a: W8.t Array32.t) (i j: int):
   0 <= j < 8 =>
   let f = f32u8_t8u32 a in
   let linear_idx = 8 * i + j in
-  let di = linear_idx %/ 32 in (* FIXME HERE *)
+  let di = linear_idx %/ 32 in
   let n = 3 - (linear_idx %% 4) in
   let k = ((linear_idx %% 32) + n) %/ 16 in
   let sl = W8.of_int (15 - (((linear_idx %% 32) + n) %% 16)) in
@@ -2593,7 +2674,7 @@ proof. admit. (*
     rewrite a_i_j_0 //=.
   rewrite W16.and0w of_sintK /smod //=.
   rewrite /inFq Sub.insubdK 1:/# pmod_small 1:/# //=.
-*)qed.
+*) qed.
 
 (* TODO: generalize *)
 lemma true_32: forall x, 0 <= x < 8 => (W8.of_int 32).[x] = (x = 5).
@@ -2613,7 +2694,7 @@ proof. admit. (*
 *)qed.
 
 lemma poly_frommsg_corr mem _p (_m : W8.t Array32.t): 
-    equiv [ Mprevec.poly_frommsg ~ EncDec_AVX2.decode1 :
+    equiv [ Mprevec.poly_frommsg ~ EncDec_AVX2.decode1_opt :
              valid_ptr _p 32 /\
              Glob.mem{1} = mem /\ to_uint ap{1} = _p /\
              load_array32 Glob.mem{1} _p = _m /\ a{2} = _m
@@ -4281,9 +4362,18 @@ qed.
 op load_array384(m : global_mem_t, p : address) : W8.t Array384.t = 
       Array384.init (fun i => m.[p + i]).
 
+
+lemma true_170: forall x, 0 <= x < 8 => (W8.of_int 170).[x] = (x %% 2 = 1).
+proof.
+  move => x x_i.
+  rewrite /of_int /= /int2bs /= /mkseq -iotaredE /=.
+  rewrite /bits2w initiE 1:x_i /=.
+  smt(@Int).
+qed.
+
 lemma poly_tobytes_corr _a (_p : address) mem : 
-    equiv [ Mprevec.poly_tobytes ~ EncDec_AVX2.encode12 :
-             pos_bound256_cxq a{1} 0 256 2 /\  lift_array256 a{1} = _a /\
+    equiv [ Mprevec.poly_tobytes ~ EncDec_AVX2.encode12_opt :
+             pos_bound256_cxq a{1} 0 256 2 /\  lift_array256 (nttpack a{1}) = _a /\
              (forall i, 0 <= i < 256 => 0 <= a{2}.[i] < q) /\
              map inFq a{2} = _a /\ valid_ptr _p 384 /\
              Glob.mem{1} = mem /\ to_uint rp{1} = _p
@@ -4296,11 +4386,10 @@ proof.
   seq 3 1 : (#{/~a{1}}pre /\
              i{1} = i{2} /\ i{1} = 0 /\
              (forall k, 0 <= k < 16 => qx16{1}.[k] = W16.of_int 3329) /\
-             map W16.to_uint a{1} = a{2} /\
+             map W16.to_uint (nttpack a{1}) = a{2} /\
              pos_bound256_cxq a{1} 0 256 1).
-  wp; call{1} (poly_csubq_corr _a); auto => />.
-  auto => />.
-  move => &1 &2 [#] pos_bound_a a2_bnd a_def rp_lb rp_ub a a1_eq_a pos_bound_an/>.
+  wp; ecall{1} (poly_csubq_corr (lift_array256 a{1})); auto => />.
+  move => &1 &2 [#] pos_bound_a a2_bnd a_def rp_lb rp_ub a a1_eq_a pos_bound_an />.
   split.
     + move => k k_lb k_ub.
       rewrite /(KyberCPA_avx2.jqx16).
@@ -4544,7 +4633,395 @@ proof.
         rewrite (pmod_small (to_uint a{1}.[128 * i{2} + 96 + k] %/ 256) 65536).
           move : (pos_ubound_a (128 * i{2} + 96 + k)) => /#.
         rewrite (pmod_small _ 16); by move : (pos_ubound_a ((128 * i{2} + 96 + k))) => /#.
-    admit. (* FIXME *)
-    admit.
+  seq 18 1: (#{~tt{1}}{~t0{1}}{~t1{1}}{~t2{1}}{~t3{1}}{~t4{1}}pre /\
+             (forall k, 0 <= k < 32 => t0_b{1}.[k] = r{2}.[192 * i{1} + k]) /\
+             (forall k, 0 <= k < 32 => t2_b{1}.[k] = r{2}.[192 * i{1} + 32 + k]) /\
+             (forall k, 0 <= k < 32 => t1_b{1}.[k] = r{2}.[192 * i{1} + 64 + k]) /\
+             (forall k, 0 <= k < 32 => t3_b{1}.[k] = r{2}.[192 * i{1} + 80 + k]) /\
+             (forall k, 0 <= k < 32 => ttt_b{1}.[k] = r{2}.[192 * i{1} + 96 + k]) /\
+             (forall k, 0 <= k < 32 => t4_b{1}.[k] = r{2}.[192 * i{1} + 112 + k])).
+  inline *; wp; skip; auto => />.
+  move => &1 &2 [#] a1_bnd p_lb p_ub qx16_def pos_bound_a i_lb i_ub touch_mem_l r2_def i_tub tt_def t0_def t1_def t2_def t3_def t4_def />.
+  do split.
+    move => k k_lb k_ub.
+    rewrite (r2_def k); first by rewrite k_lb k_ub.
+    rewrite filliE 1:/#.
+    rewrite lezNgt k_ub //=.
+
+    move => k k_lb k_ub.
+    rewrite /f16u16_t32u8 /f8u32_t16u16 /f16u16_t8u32 /f4u64_t16u16 /f16u16_t4u64.
+    do (rewrite initiE 1:/# //= || rewrite mapiE 1:/# //=).
+    have ->: !W8.int_bit 32 (4 * (k %/ 2 %/ 8) + 3).
+      move : (true_32 (4 * (k %/ 2 %/ 8) + 3)).
+      rewrite of_intwE.
+      smt(@Int @IntDiv).
+    have -> //=: !W8.int_bit 32 (4 * (k %/ 2 %/ 8)).
+      move : (true_32 (4 * (k %/ 2 %/ 8))).
+      rewrite of_intwE.
+      smt(@Int @IntDiv).
+    have -> //=: (0 <= 4 * (k %/ 2 %/ 8) + 1 && 4 * (k %/ 2 %/ 8) + 1 < 8).
+      move : k_lb k_ub; smt(@Int @IntDiv).
+    rewrite (_ : W8.int_bit 32 (4 * (k %/ 2 %/ 8) + 1) = (k %/ 16 = 1)).
+      move : (true_32 (4 * (k %/ 2 %/ 8) + 1)).
+      rewrite of_intwE.
+      smt(@Int @IntDiv).
+    do rewrite fun_if2.
+    do (rewrite initiE 1:/# //= || rewrite mapiE 1:/# //=).
+    rewrite (pdiv_small (k %/ 2 %% 8) 8) 1:modz_cmp //=.
+    rewrite (pdiv_small (k %/ 2 %% 8 %% 4) 4) 1:modz_cmp //=.
+    do (rewrite (modz_cmp _ 8) 1://= //=).
+    do (rewrite (modz_dvd _ _ 4) 1://= || rewrite (modz_dvd _ _ 2) 1://=).
+    rewrite (pdiv_small (k %/ 2 %% 2) 2) 1:modz_cmp //=.
+    rewrite (pmod_small (k %/ 2 %% 4) 8) 1:/# //=.
+    rewrite (pmod_small (k %/ 2 %% 2) 8) 1:/# //=.
+    have -> //=: (0 <= k %/ 2 %% 4 %/ 2 && k %/ 2 %% 4 %/ 2 < 8). move : (modz_cmp (k %/ 2) 4) => /#.
+    rewrite (_: k %/ 2 %% 4 %/ 2 = k %/ 4 %% 2). smt(@Int @IntDiv modz_pow2_div).
+    rewrite (_: k %/ 2 %% 8 %/ 4 %% 2 = k %/ 8 %% 2). smt(@Int @IntDiv modz_pow2_div).
+    rewrite (_: W8.int_bit 170 (k %/ 4 %% 2) = (k %/ 4 %% 2 = 1)).
+      move : (true_170 (k %/ 4 %% 2)).
+      rewrite of_intwE.
+      smt(@Int @IntDiv).
+    rewrite (_: W8.int_bit 170 (k %/ 2 %% 2) = (k %/ 2 %% 2 = 1)).
+      move : (true_170 (k %/ 2 %% 2)).
+      rewrite of_intwE.
+      smt(@Int @IntDiv).
+    rewrite (_: W8.int_bit 170 (k %/ 2 %% 4) = (k %/ 2 %% 2 = 1)).
+      move : (true_170 (k %/ 2 %% 4)).
+      rewrite of_intwE.
+      smt(@Int @IntDiv).
+    rewrite filliE 1://#.
+    have -> //=: 192 * i{2} <= 192 * i{2} + k && 192 * i{2} + k < 192 * i{2} + 192.
+      move : k_ub k_lb => /#.
+  rewrite (_: (if k %/ 4 %% 2 = 1 then
+                 if k %/ 2 %% 2 = 1 then t4{1}.[k %/ 2 %% 2]
+                 else
+                   pack2_t ((init ("_.[_]" t3{1})))%W2u16.Pack `>>` (of_int 16)%W8 \bits16
+                   k %/ 2 %% 2
+               else
+                 if k %/ 2 %% 2 = 1 then t2{1}.[k %/ 2 %% 4]
+                 else
+                   pack2_t
+                     ((init (fun (j : int) => t1{1}.[2 * (k %/ 4 %% 2) + j])))%W2u16.Pack `>>`
+                   (of_int 16)%W8 \bits16 k %/ 2 %% 2) =
+              (if k %/ 4 %% 2 = 1 then
+                 if k %/ 2 %% 2 = 1 then t4{1}.[1]
+                 else
+                   pack2_t ((init ("_.[_]" t3{1})))%W2u16.Pack `>>` (of_int 16)%W8 \bits16 0
+               else
+                 if k %/ 2 %% 2 = 1 then t2{1}.[1]
+                 else
+                   pack2_t
+                     ((init (fun (j : int) => t1{1}.[j])))%W2u16.Pack `>>`
+                   (of_int 16)%W8 \bits16 0)).
+    case (k %/ 4 %% 2 = 1) => if_1_t.
+      + smt(@Logic).
+      + have ->: k %/ 4 %% 2 = 0. move : if_1_t (modz_cmp (k %/ 4) 2) => /#.
+        case (k %/ 2 %% 2 = 1) => if_2_t.
+          move : if_1_t if_2_t; smt(@Int @IntDiv).
+          have ->: k %/ 2 %% 2 = 0. move : if_2_t (modz_cmp (k %/ 2) 2) => /#.
+          trivial.
+  rewrite (_: (if k %/ 4 %% 2 = 1 then
+                 if k %/ 2 %% 2 = 1 then
+                   pack2_t
+                     ((init (fun (j : int) => t2{1}.[2 * (k %/ 4 %% 2) + j])))%W2u16.Pack `<<`
+                   (of_int 16)%W8 \bits16 k %/ 2 %% 2
+                 else t1{1}.[k %/ 2 %% 4]
+               else
+                 pack4_t
+                   ((init
+                       ("_.[_]"
+                          ((init
+                              (fun (i0 : int) =>
+                                 if (0 <= i0 %% 8 && i0 %% 8 < 8) /\
+                                    (int_bit 170 (i0 %% 8))%W8 then
+                                   ((init
+                                       (fun (i1 : int) =>
+                                          ((init
+                                              (fun (i2 : int) =>
+                                                 ((init
+                                                     (fun (i3 : int) =>
+                                                        pack2_t
+                                                          ((init
+                                                              (fun (j : int) =>
+                                                                 t0{1}.[2 * i3 + j])))%W2u16.Pack)))%Array8.[i2] `<<`
+                                                 (of_int 16)%W8)))%Array8.[i1 %/ 2] \bits16
+                                          i1 %% 2)))%Array16.[i0]
+                                 else tt{1}.[i0])))%Array16)))%W4u16.Pack `>>`
+                 (of_int 32)%W8 \bits16 k %/ 2 %% 4) =
+              (if k %/ 4 %% 2 = 1 then
+                 if k %/ 2 %% 2 = 1 then
+                   pack2_t
+                     ((init (fun (j : int) => t2{1}.[2 + j])))%W2u16.Pack `<<`
+                   (of_int 16)%W8 \bits16 1
+                 else t1{1}.[2]
+               else
+                 pack4_t
+                   ((init
+                       ("_.[_]"
+                          ((init
+                              (fun (i0 : int) =>
+                                 if (0 <= i0 %% 8 && i0 %% 8 < 8) /\
+                                    (int_bit 170 (i0 %% 8))%W8 then
+                                   ((init
+                                       (fun (i1 : int) =>
+                                          ((init
+                                              (fun (i2 : int) =>
+                                                 ((init
+                                                     (fun (i3 : int) =>
+                                                        pack2_t
+                                                          ((init
+                                                              (fun (j : int) =>
+                                                                 t0{1}.[2 * i3 + j])))%W2u16.Pack)))%Array8.[i2] `<<`
+                                                 (of_int 16)%W8)))%Array8.[i1 %/ 2] \bits16
+                                          i1 %% 2)))%Array16.[i0]
+                                 else tt{1}.[i0])))%Array16)))%W4u16.Pack `>>`
+                 (of_int 32)%W8 \bits16 k %/ 2 %% 4)).
+    case (k %/ 4 %% 2 = 1) => if_1_t.
+      + case (k %/ 2 %% 2 = 1) => if_2_t.
+          rewrite if_1_t if_2_t //=.
+          move : if_1_t if_2_t; smt(@Int @IntDiv).
+      + done.
+  do (rewrite (fun_if2 (W2u8.\bits8))).
+  do rewrite (mulzC 192 i{2}).
+  rewrite modzMDl.
+  do (rewrite mapiE 1:/# //=).
+  do (rewrite shl_shlw 1://= || rewrite shr_shrw 1://=).
+  pose t3_pack := pack2_t ((W2u16.Pack.init ("_.[_]" t3{1}))).
+  pose t1_pack := pack2_t ((W2u16.Pack.init ("_.[_]" t1{1}))).
+  pose t2_pack := pack2_t ((W2u16.Pack.init (fun (j : int) => t2{1}.[2 + j]))).
+  rewrite -(W32.to_uintK t3_pack) -(W32.to_uintK t1_pack) -(W32.to_uintK t2_pack).
+  rewrite shrDP 1://= (pmod_small _ W32.modulus) 1:W32.to_uint_cmp.
+  rewrite shrDP 1://= (pmod_small _ W32.modulus) 1:W32.to_uint_cmp.
+  rewrite (_: W16.modulus = 2 ^ (16 * 1)). by trivial.
+  do (rewrite of_int_bits16_div 1://=).
+  do (rewrite -divzMr 1..2://=).
+  rewrite -exprD_nneg 1..2://=.
+  do rewrite -(mulzDr 16 _ _).
+  do (rewrite -W2u16.of_int_bits16_div 1://=).
+  rewrite addz0 to_uintK -(W2u16.get_unpack16 _ 1) 1://= pack2K initiE 1://=.
+  rewrite to_uintK -(W2u16.get_unpack16 _ 1) 1://= pack2K initiE 1://=.
+
+  rewrite shlMP 1://=.
+  rewrite of_int_bits16_div 1://=.
+  rewrite (_: to_uint t2_pack * W16.modulus %/ 2 ^ (16 * 1) = to_uint t2_pack %/ 2 ^ (16 * 0)).
+    by rewrite expr0 mulzK 1://= divz1.
+  rewrite -W2u16.of_int_bits16_div 1://=.
+  rewrite to_uintK -(W2u16.get_unpack16 _ 0) 1://= pack2K initiE 1://= //=.
+  pose tt_t0_pack := pack4_t
+     ((W4u16.Pack.init
+         ("_.[_]"
+            ((init
+                (fun (i0 : int) =>
+                   if (0 <= i0 %% 8 && i0 %% 8 < 8) /\
+                      (int_bit 170 (i0 %% 8))%W8 then
+                     ((init
+                         (fun (i1 : int) =>
+                            ((init
+                                (fun (i2 : int) =>
+                                   ((init
+                                       (fun (i3 : int) =>
+                                          pack2_t
+                                            ((init
+                                                (fun (j : int) =>
+                                                   t0{1}.[2 * i3 + j])))%W2u16.Pack)))%Array8.[i2] `<<`
+                                   (of_int 16)%W8)))%Array8.[i1 %/ 2] \bits16
+                            i1 %% 2)))%Array16.[i0]
+                   else tt{1}.[i0])))%Array16))).
+  rewrite -(W64.to_uintK tt_t0_pack).  
+  rewrite shrDP 1://= (pmod_small _ W64.modulus) 1:W64.to_uint_cmp.
+  rewrite of_int_bits16_div 1:modz_cmp 1://=.
+  rewrite -divzMr 1://=. move : (modz_cmp k 4); smt(@Int @IntDiv @Ring.IntID).
+  rewrite -exprD_nneg 1://=. smt(@Int @IntDiv @Ring.IntID).
+  rewrite (_: 32 = 16 * 2) 1://= -(mulzDr 16 _ _).
+  rewrite (_: (if k %/ 8 %% 2 = 0 then
+                 if k %/ 4 %% 2 = 1 then
+                   if k %/ 2 %% 2 = 1 then t4{1}.[1] \bits8 k %% 2
+                   else t3{1}.[1] \bits8 k %% 2
+                 else
+                   if k %/ 2 %% 2 = 1 then t2{1}.[1] \bits8 k %% 2
+                   else t1{1}.[1] \bits8 k %% 2
+               else
+                 if k %/ 4 %% 2 = 1 then
+                   if k %/ 2 %% 2 = 1 then t2{1}.[2] \bits8 k %% 2
+                   else t1{1}.[2] \bits8 k %% 2
+                 else
+                  (of_int (to_uint tt_t0_pack %/ 2 ^ (16 * (2 + k %/ 2 %% 4))))%W16 \bits8
+                  k %% 2) =
+              (if k %/ 8 %% 2 = 0 then
+                 if k %/ 4 %% 2 = 1 then
+                   if k %/ 2 %% 2 = 1 then t4{1}.[1] \bits8 k %% 2
+                   else t3{1}.[1] \bits8 k %% 2
+                 else
+                   if k %/ 2 %% 2 = 1 then t2{1}.[1] \bits8 k %% 2
+                   else t1{1}.[1] \bits8 k %% 2
+               else
+                 if k %/ 4 %% 2 = 1 then
+                   if k %/ 2 %% 2 = 1 then t2{1}.[2] \bits8 k %% 2
+                   else t1{1}.[2] \bits8 k %% 2
+                 else
+                  (of_int (to_uint tt_t0_pack %/ 2 ^ (16 * (2 + k %/ 2 %% 2))))%W16 \bits8
+                  k %% 2)).
+    case (k %/ 8 %% 2 = 0) => />.
+      + move => if_1_f.
+        case (k %/ 4 %% 2 = 1) => />.
+          + move => if_2_f.
+            have if_1_fv: k %/ 8 %% 2 = 1. move : if_1_f (modz_cmp (k %/ 8) 2) => /#.
+            have if_2_fv: k %/ 4 %% 2 = 0. move : if_2_f (modz_cmp (k %/ 4) 2) => /#.
+            have ->: k %/ 2 %% 4 = k %/ 2 %% 2. move : if_2_fv if_1_fv; smt(@Int @IntDiv).
+            done.
+  rewrite -W4u16.of_int_bits16_div; first by move : (modz_cmp (k %/ 2) 2) => /#.
+  rewrite to_uintK -W4u16.get_unpack16 1:/# pack4K.
+  do (rewrite initiE 1:/# //=).
+  rewrite (modz_cmp _ 8) 1://= //=.
+  rewrite (_: 2 * ((2 + k %/ 2 %% 2) %/ 2) = 2).
+    rewrite -(mul1z 2) divzMDl //= (pdiv_small (k %/ 2 %% 2) 2) 1:modz_cmp //=.
+  rewrite (_: (2 + k %/ 2 %% 2) %% 2 = k %/ 2 %% 2). smt(@Int @IntDiv modz_mod).
+  pose t0_pack := pack2_t ((W2u16.Pack.init (fun (j : int) => t0{1}.[2 + j]))).
+  rewrite -(W32.to_uintK t0_pack).
+  rewrite shl_shlw 1://= shlMP 1://=.
+  rewrite of_int_bits16_div 1:/#.
+  rewrite (_: W16.modulus = 2 ^ (16 * 1)). by trivial.
+  rewrite (_: W8.int_bit 170 ((2 + k %/ 2 %% 2) %% 8) = (k %/ 2 %% 2 = 1)).
+    move : (true_170 ((2 + k %/ 2 %% 2) %% 8)).
+    rewrite of_intwE.
+    smt(@Int @IntDiv).
+  rewrite (fun_if2 (W2u8.\bits8)).
+  rewrite (_: (if k %/ 2 %% 2 = 1 then
+                 (W16.of_int (to_uint t0_pack * 2 ^ (16 * 1) %/ 2 ^ (16 * (k %/ 2 %% 2)))) \bits8 k%% 2
+               else tt{1}.[2 + k %/ 2 %% 2] \bits8 k %% 2) =
+              (if k %/ 2 %% 2 = 1 then
+                 (W16.of_int (to_uint t0_pack * 2 ^ (16 * 1) %/ 2 ^ (16 * 1))) \bits8 k%% 2
+               else tt{1}.[2] \bits8 k %% 2)).
+    case (k %/ 2 %% 2 = 1) => if_1_t.
+      rewrite if_1_t //=.
+      have -> //=: k %/ 2 %% 2 = 0. move : if_1_t => /#.
+  rewrite (_: to_uint t0_pack * W16.modulus %/ 2 ^ (16 * 1) = to_uint t0_pack %/ 2 ^ (16 * 0)).
+    by rewrite expr0 mulzK 1://= divz1.
+  rewrite -W2u16.of_int_bits16_div 1://=.
+  rewrite to_uintK -(W2u16.get_unpack16 _ 0) 1://= pack2K initiE 1://= //=.
+  do (rewrite bits8_div 1:/#).
+
+  rewrite (_: (if k %/ 8 %% 2 = 0 then
+                 if k %/ 4 %% 2 = 1 then
+                   if k %/ 2 %% 2 = 1 then
+                     (of_int
+                        (to_uint
+                           (pack2_t ((W2u16.Pack.init ("_.[_]" t2{1}))) `<<<` 16 \bits16 k %/ 2 %% 2) %/
+                         2 ^ (8 * (k %% 2))))%W8
+                   else (of_int (to_uint t1{1}.[k %/ 2 %% 2] %/ 2 ^ (8 * (k %% 2))))%W8
+                 else
+                   if k %/ 2 %% 2 = 1 then
+                     (of_int
+                        (to_uint
+                           (pack2_t
+                              ((init (fun (j : int) => t0{1}.[2 * (k %/ 4 %% 2) + j])))%W2u16.Pack `<<<`
+                            16 \bits16 k %/ 2 %% 2) %/
+                         2 ^ (8 * (k %% 2))))%W8
+                   else (of_int (to_uint tt{1}.[k %/ 2 %% 4] %/ 2 ^ (8 * (k %% 2))))%W8
+               else
+                 if k %/ 4 %% 2 = 1 then
+                   if k %/ 2 %% 2 = 1 then
+                     (of_int (to_uint t0{1}.[k %/ 2 %% 2] %/ 2 ^ (8 * (k %% 2))))%W8
+                   else
+                     (of_int
+                        (to_uint
+                           (pack2_t ((init ("_.[_]" tt{1})))%W2u16.Pack `>>>` 16 \bits16
+                            k %/ 2 %% 2) %/
+                         2 ^ (8 * (k %% 2))))%W8
+                 else
+                   if k %/ 2 %% 2 = 1 then
+                     (of_int
+                        (to_uint
+                           (pack2_t
+                              ((init (fun (j : int) => t4{1}.[2 * (k %/ 4 %% 2) + j])))%W2u16.Pack `<<<`
+                            16 \bits16 k %/ 2 %% 2) %/
+                         2 ^ (8 * (k %% 2))))%W8
+                   else (of_int (to_uint t3{1}.[k %/ 2 %% 4] %/ 2 ^ (8 * (k %% 2))))%W8) =
+              (if k %/ 8 %% 2 = 0 then
+                 if k %/ 4 %% 2 = 1 then
+                   if k %/ 2 %% 2 = 1 then
+                     (of_int
+                        (to_uint
+                           (pack2_t ((W2u16.Pack.init ("_.[_]" t2{1}))) `<<<` 16 \bits16 1) %/ 2 ^ (8 * (k %% 2))))%W8
+                   else (of_int (to_uint t1{1}.[0] %/ 2 ^ (8 * (k %% 2))))%W8
+                 else
+                   if k %/ 2 %% 2 = 1 then
+                     (of_int
+                        (to_uint
+                           (pack2_t
+                              ((W2u16.Pack.init (fun (j : int) => t0{1}.[j]))) `<<<` 16 \bits16 1) %/ 2 ^ (8 * (k %% 2))))%W8
+                   else (of_int (to_uint tt{1}.[0] %/ 2 ^ (8 * (k %% 2))))%W8
+               else
+                 if k %/ 4 %% 2 = 1 then
+                   if k %/ 2 %% 2 = 1 then
+                     (of_int (to_uint t0{1}.[1] %/ 2 ^ (8 * (k %% 2))))%W8
+                   else
+                     (of_int
+                        (to_uint
+                           (pack2_t ((W2u16.Pack.init ("_.[_]" tt{1}))) `>>>` 16 \bits16 0) %/ 2 ^ (8 * (k %% 2))))%W8
+                 else
+                   if k %/ 2 %% 2 = 1 then
+                     (of_int
+                        (to_uint
+                           (pack2_t
+                              ((W2u16.Pack.init (fun (j : int) => t4{1}.[j]))) `<<<` 16 \bits16 1) %/ 2 ^ (8 * (k %% 2))))%W8
+                   else (of_int (to_uint t3{1}.[0] %/ 2 ^ (8 * (k %% 2))))%W8)).
+    case(k %/ 8 %% 2 = 0) => if_1_t.
+      case (k %/ 4 %% 2 = 1) => if_2_t.
+        + smt(@Logic @Int @IntDiv).
+        + have -> //=: k %/ 4 %% 2 = 0. move : if_2_t (modz_cmp (k %/ 4) 2 ) => /#.
+          have ->: k %/ 2 %% 4 = k %/ 2 %% 2. move : if_2_t if_1_t; smt(@Int @IntDiv).
+          smt(@Logic @Int @IntDiv).
+      case (k %/ 4 %% 2 = 1) => if_2_t.
+        + smt(@Logic @Int @IntDiv).
+        + have -> //=: k %/ 4 %% 2 = 0. move : if_2_t (modz_cmp (k %/ 4) 2 ) => /#.
+          have ->: k %/ 2 %% 4 = k %/ 2 %% 2. move : if_2_t if_1_t; smt(@Int @IntDiv).
+          smt(@Logic @Int @IntDiv).
+  move : t3_pack t1_pack t2_pack tt_t0_pack t0_pack => _ _ _ _ _.
+  pose t0_pack := pack2_t ((W2u16.Pack.init (fun (j : int) => t0{1}.[j]))).
+  pose t2_pack := pack2_t ((W2u16.Pack.init ("_.[_]" t2{1}))).
+  pose t4_pack := pack2_t ((W2u16.Pack.init (fun (j : int) => t4{1}.[j]))).
+  pose tt_pack := pack2_t ((W2u16.Pack.init ("_.[_]" tt{1}))).
+  rewrite -(W32.to_uintK t0_pack) -(W32.to_uintK t2_pack) -(W32.to_uintK t4_pack) -(W32.to_uintK tt_pack).
+  rewrite shrDP 1://= (pmod_small _ W32.modulus) 1:W32.to_uint_cmp.
+  do (rewrite shlMP 1://=).
+  rewrite (_: W16.modulus = 2 ^ (16 * 1)). by trivial.
+  do (rewrite of_int_bits16_div 1://=).
+  have H: forall (t: int), t * 2 ^ (16 * 1) %/ 2 ^ (16 * 1) = t %/ 2 ^ (16 * 0).
+    by move => t; rewrite expr0 mulzK 1://= divz1.
+  do rewrite H.
+  do (rewrite -divzMr 1..2://=).
+  rewrite -exprD_nneg 1..2://=.
+  do rewrite -(mulzDr 16 _ _).
+  do (rewrite -W2u16.of_int_bits16_div 1://=).
+  rewrite addz0.
+  rewrite (W32.to_uintK t2_pack) -(W2u16.get_unpack16 _ 0) 1://= pack2K initiE 1://=.
+  rewrite (W32.to_uintK t0_pack) -(W2u16.get_unpack16 _ 0) 1://= pack2K initiE 1://=.
+  rewrite (W32.to_uintK tt_pack) -(W2u16.get_unpack16 _ 1) 1://= pack2K initiE 1://=.
+  rewrite (W32.to_uintK t4_pack) -(W2u16.get_unpack16 _ 0) 1://= pack2K initiE 1://= //=.
+
+  (* HERE: repeat for other half *)
+  do (rewrite t4_def 1://= || rewrite t3_def 1://= || rewrite t2_def 1://= ||
+      rewrite t1_def 1://= || rewrite t0_def 1://= || rewrite tt_def 1://=).
+  have k_iota: k \in (iota_ 0 32); first by rewrite mem_iota k_lb k_ub.
+  rewrite (pmod_small k 192); first by move : k_lb k_ub => /#.
+  rewrite (_: i{2} * 192 = (i{2} * 64) * 3); first by ring.
+  rewrite (modzMDl _ _ 3).
+  do (rewrite mapiE; first by move : i_lb i_tub => /#).
+  rewrite /pos_bound256_cxq /bpos16 //= in pos_bound_a.
+  have pos_ubound_a: forall (k : int), 0 <= k && k < 256 => 0 <= to_uint a{1}.[k] && to_uint a{1}.[k] < q.
+    move => j j_i.
+    rewrite -to_sint_unsigned.
+    move : (pos_bound_a j j_i) => />.
+    apply (pos_bound_a j j_i).
+  do (rewrite inFqK (pmod_small _ q) 1:pos_ubound_a 1:/#).
+  case (k = 1) => k_1.
+    rewrite k_1 //=.
+    smt(@Int @IntDiv @Array384 @W16 @W8 @Ring.IntID @W32 @List @Logic).
+    move : H.
+    rewrite -iotaredE /=.
+    case
+    smt(@Int @IntDiv @Array384 @W16 @W8 @Ring.IntID @W32 @List).
+
 qed.
 end KyberPolyAVX.
